

My article

Wei October 24, 2025

$$\lambda = (a, -c, b|b)$$

$$\mathbf{1} \quad b < c \leq a$$

$$\mathbf{1.1} \quad b + 1 < c$$

$$pr_{\lambda}(P_{a,-c,b+1|b} \otimes V) = \sum(a, -c, b, b) + \sum(a, -c, b + 1, b + 1)$$

$$\mathbf{1.2} \quad b + 1 = c \quad \lambda = (a, b - 1, b, b)$$

$$\mathbf{1.2.1} \quad a > c$$

$$pr_{\lambda}(P_{a,-b-1,b+1|b} \otimes V) = \sum(a, -b - 1, b, b) + \sum(a, -b - 1, b + 1, b + 1)$$

$$\mathbf{1.2.2} \quad a = c$$

$$pr_{\lambda}(P_{b+2,-b-1,b+1|b} \otimes V) = \sum M(b + 2, -b - 1, b, b) + \sum M(b + 2, -b - 1, b + 1, b + 1) + \sum M(b + 2, -b - 1, b + 1, b + 2)$$